add b

VST-introduction/get_global_pointer.c
@@ -19,3 +19,36 @@ int i;
 int get_i() {
   return i;
 }
+
+// working in progress
+
+struct a {int x1; int x2;};
+struct b {int y1; struct node *innerlist;};
+
+struct b p;
+
+int get(void) {
+  return p.y1;
+}
+
+
+
+
+
+
+
+// not verified_
+
+
+struct {
+  int xx; // lock
+  struct node *innerlist;
+} kmem;
+
+struct node *get_innerlist() {
+  return kmem.innerlist;
+}
+
+int get_xx_2() {
+  return kmem.xx;
+}
